\documentclass{article}
\usepackage[T2A]{fontenc}
\usepackage[utf8]{inputenc}
\usepackage[russian]{babel}
\usepackage{amsmath}
\usepackage{graphicx}
\usepackage[legalpaper, landscape, margin=1in]{geometry}
\begin{document}
\allowdisplaybreaks
\begin{gather*}
{{\frac{{d}}{{d{{x}}}}}{{{\frac{{d}}{{d{{x}}}}}{{{{x}^{2}}{\left(\ln{{x}}\right)}}}}}}=\\
={{\frac{{d}}{{d{{x}}}}}{{{\frac{{d}}{{d{{x}}}}}{{{\left(\ln{{x}}\right)}{{x}^{2}}}}}}}=\\
={{\frac{{d}}{{d{{x}}}}}{{\left({{\left(\ln{{x}}\right)}{\left({\frac{{d}}{{d{{x}}}}}{{{x}^{2}}}\right)}}+{{\left({\frac{{d}}{{d{{x}}}}}{{\ln{{x}}}}\right)}{{x}^{2}}}\right)}}}=\\
={{\frac{{d}}{{d{{x}}}}}{{\left({{\left(\ln{{x}}\right)}{{\left({\frac{{d}}{{d{{x}}}}}{{x}}\right)}{\cdot}{{2}{{x}^{1}}}}}+{{\left({\frac{{d}}{{d{{x}}}}}{{\ln{{x}}}}\right)}{{x}^{2}}}\right)}}}=\\
={{\frac{{d}}{{d{{x}}}}}{{\left({{\left(\ln{{x}}\right)}{\cdot}{{1}{\cdot}{{2}{{x}^{1}}}}}+{{\left({\frac{{d}}{{d{{x}}}}}{{\ln{{x}}}}\right)}{{x}^{2}}}\right)}}}=\\
={{\frac{{d}}{{d{{x}}}}}{{\left({{\left(\ln{{x}}\right)}{\cdot}{{1}{\cdot}{{2}{x}}}}+{{\left({\frac{{d}}{{d{{x}}}}}{{\ln{{x}}}}\right)}{{x}^{2}}}\right)}}}=\\
={{\frac{{d}}{{d{{x}}}}}{{\left({{\left(\ln{{x}}\right)}{\cdot}{{1}{{x}{\cdot}{2}}}}+{{\left({\frac{{d}}{{d{{x}}}}}{{\ln{{x}}}}\right)}{{x}^{2}}}\right)}}}=\\
={{\frac{{d}}{{d{{x}}}}}{{\left({{\left(\ln{{x}}\right)}{{x}{\cdot}{{2}{\cdot}{1}}}}+{{\left({\frac{{d}}{{d{{x}}}}}{{\ln{{x}}}}\right)}{{x}^{2}}}\right)}}}=\\
={{\frac{{d}}{{d{{x}}}}}{{\left({{\left(\ln{{x}}\right)}{{x}{\cdot}{2}}}+{{\left({\frac{{d}}{{d{{x}}}}}{{\ln{{x}}}}\right)}{{x}^{2}}}\right)}}}=\\
={{\frac{{d}}{{d{{x}}}}}{{\left({{\left(\ln{{x}}\right)}{{x}{\cdot}{2}}}+{{\left({\frac{{d}}{{d{{x}}}}}{{x}}\right)}{\cdot}{{\left(\frac{{1}}{{x}}\right)}{{x}^{2}}}}\right)}}}=\\
={{\frac{{d}}{{d{{x}}}}}{{\left({{\left(\ln{{x}}\right)}{{x}{\cdot}{2}}}+{{1}{\cdot}{{\left(\frac{{1}}{{x}}\right)}{{x}^{2}}}}\right)}}}=\\
={{\frac{{d}}{{d{{x}}}}}{{\left({{\left(\ln{{x}}\right)}{{x}{\cdot}{2}}}+{{1}{\cdot}{\left(\frac{{{1}{{x}^{2}}}}{{x}}\right)}}\right)}}}=\\
={{\frac{{d}}{{d{{x}}}}}{{\left({{\left(\ln{{x}}\right)}{{x}{\cdot}{2}}}+{{1}{\left(\frac{{{{x}^{2}}{\cdot}{1}}}{{x}}\right)}}\right)}}}=\\
={{\frac{{d}}{{d{{x}}}}}{{\left({{\left(\ln{{x}}\right)}{{x}{\cdot}{2}}}+{{1}{\left(\frac{{{x}^{2}}}{{x}}\right)}}\right)}}}=\\
={{\frac{{d}}{{d{{x}}}}}{{\left({{\left(\ln{{x}}\right)}{{x}{\cdot}{2}}}+{{1}{\cdot}{\left(\frac{{{{1}^{2}}{{x}^{\left({2}-{{1}{\cdot}{1}}\right)}}}}{{{1}{{x}^{\left({1}-{{1}{\cdot}{1}}\right)}}}}\right)}}\right)}}}=\\
={{\frac{{d}}{{d{{x}}}}}{{\left({{\left(\ln{{x}}\right)}{{x}{\cdot}{2}}}+{{1}{\cdot}{\left(\frac{{{1}{{x}^{\left({2}-{{1}{\cdot}{1}}\right)}}}}{{{1}{{x}^{\left({1}-{{1}{\cdot}{1}}\right)}}}}\right)}}\right)}}}=\\
={{\frac{{d}}{{d{{x}}}}}{{\left({{\left(\ln{{x}}\right)}{{x}{\cdot}{2}}}+{{1}{\cdot}{\left(\frac{{{1}{{x}^{\left({2}-{1}\right)}}}}{{{1}{{x}^{\left({1}-{{1}{\cdot}{1}}\right)}}}}\right)}}\right)}}}=\\
={{\frac{{d}}{{d{{x}}}}}{{\left({{\left(\ln{{x}}\right)}{{x}{\cdot}{2}}}+{{1}{\cdot}{\left(\frac{{{1}{{x}^{\left({-{1}}+{2}\right)}}}}{{{1}{{x}^{\left({1}-{{1}{\cdot}{1}}\right)}}}}\right)}}\right)}}}=\\
={{\frac{{d}}{{d{{x}}}}}{{\left({{\left(\ln{{x}}\right)}{{x}{\cdot}{2}}}+{{1}{\cdot}{\left(\frac{{{1}{x}}}{{{1}{{x}^{\left({1}-{{1}{\cdot}{1}}\right)}}}}\right)}}\right)}}}=\\
={{\frac{{d}}{{d{{x}}}}}{{\left({{\left(\ln{{x}}\right)}{{x}{\cdot}{2}}}+{{1}{\left(\frac{{{x}{\cdot}{1}}}{{{1}{{x}^{\left({1}-{{1}{\cdot}{1}}\right)}}}}\right)}}\right)}}}=\\
={{\frac{{d}}{{d{{x}}}}}{{\left({{\left(\ln{{x}}\right)}{{x}{\cdot}{2}}}+{{1}{\left(\frac{{x}}{{{1}{{x}^{\left({1}-{{1}{\cdot}{1}}\right)}}}}\right)}}\right)}}}=\\
={{\frac{{d}}{{d{{x}}}}}{{\left({{\left(\ln{{x}}\right)}{{x}{\cdot}{2}}}+{{1}{\left(\frac{{x}}{{{1}{{x}^{\left({1}-{1}\right)}}}}\right)}}\right)}}}=\\
={{\frac{{d}}{{d{{x}}}}}{{\left({{\left(\ln{{x}}\right)}{{x}{\cdot}{2}}}+{{1}{\left(\frac{{x}}{{{1}{{x}^{\left({-{1}}+{1}\right)}}}}\right)}}\right)}}}=\\
={{\frac{{d}}{{d{{x}}}}}{{\left({{\left(\ln{{x}}\right)}{{x}{\cdot}{2}}}+{{1}{\left(\frac{{x}}{{{1}{{x}^{\left(-{0}\right)}}}}\right)}}\right)}}}=\\
={{\frac{{d}}{{d{{x}}}}}{{\left({{\left(\ln{{x}}\right)}{{x}{\cdot}{2}}}+{{1}{x}}\right)}}}=\\
={{\frac{{d}}{{d{{x}}}}}{{\left({{\left(\ln{{x}}\right)}{{x}{\cdot}{2}}}+{{x}{\cdot}{1}}\right)}}}=\\
={{\frac{{d}}{{d{{x}}}}}{{\left({{\left(\ln{{x}}\right)}{{x}{\cdot}{2}}}+{x}\right)}}}=\\
={{\frac{{d}}{{d{{x}}}}}{{{{x}^{\left({1}{\cdot}{1}\right)}}{\left({{{\left(\ln{{x}}\right)}{\cdot}{{1}{\cdot}{2}}}{{x}^{\left({1}-{{1}{\cdot}{1}}\right)}}}+{{1}{{x}^{\left({1}-{{1}{\cdot}{1}}\right)}}}\right)}}}}=\\
={{\frac{{d}}{{d{{x}}}}}{{{x}{\left({{{\left(\ln{{x}}\right)}{\cdot}{{1}{\cdot}{2}}}{{x}^{\left({1}-{{1}{\cdot}{1}}\right)}}}+{{1}{{x}^{\left({1}-{{1}{\cdot}{1}}\right)}}}\right)}}}}=\\
={{\frac{{d}}{{d{{x}}}}}{{{x}{\left({{\left(\ln{{x}}\right)}{\cdot}{{2}{\cdot}{{1}{{x}^{\left({1}-{{1}{\cdot}{1}}\right)}}}}}+{{1}{{x}^{\left({1}-{{1}{\cdot}{1}}\right)}}}\right)}}}}=\\
={{\frac{{d}}{{d{{x}}}}}{{{x}{\left({{\left(\ln{{x}}\right)}{\cdot}{{2}{\cdot}{{1}{{x}^{\left({1}-{1}\right)}}}}}+{{1}{{x}^{\left({1}-{{1}{\cdot}{1}}\right)}}}\right)}}}}=\\
={{\frac{{d}}{{d{{x}}}}}{{{x}{\left({{\left(\ln{{x}}\right)}{\cdot}{{2}{\cdot}{{1}{{x}^{\left({-{1}}+{1}\right)}}}}}+{{1}{{x}^{\left({1}-{{1}{\cdot}{1}}\right)}}}\right)}}}}=\\
={{\frac{{d}}{{d{{x}}}}}{{{x}{\left({{\left(\ln{{x}}\right)}{\cdot}{{2}{\cdot}{{1}{{x}^{\left(-{0}\right)}}}}}+{{1}{{x}^{\left({1}-{{1}{\cdot}{1}}\right)}}}\right)}}}}=\\
={{\frac{{d}}{{d{{x}}}}}{{{x}{\left({{\left(\ln{{x}}\right)}{\cdot}{2}}+{{1}{{x}^{\left({1}-{{1}{\cdot}{1}}\right)}}}\right)}}}}=\\
={{\frac{{d}}{{d{{x}}}}}{{{x}{\left({{\left(\ln{{x}}\right)}{\cdot}{2}}+{{1}{{x}^{\left({1}-{1}\right)}}}\right)}}}}=\\
={{\frac{{d}}{{d{{x}}}}}{{{x}{\left({{\left(\ln{{x}}\right)}{\cdot}{2}}+{{1}{{x}^{\left({-{1}}+{1}\right)}}}\right)}}}}=\\
={{\frac{{d}}{{d{{x}}}}}{{{x}{\left({{\left(\ln{{x}}\right)}{\cdot}{2}}+{{1}{{x}^{\left(-{0}\right)}}}\right)}}}}=\\
={{\frac{{d}}{{d{{x}}}}}{{{x}{\left({{\left(\ln{{x}}\right)}{\cdot}{2}}+{1}\right)}}}}=\\
={{\frac{{d}}{{d{{x}}}}}{{{\left({{\left(\ln{{x}}\right)}{\cdot}{2}}+{1}\right)}{x}}}}=\\
={{{\left({{\left(\ln{{x}}\right)}{\cdot}{2}}+{1}\right)}{\left({\frac{{d}}{{d{{x}}}}}{{x}}\right)}}+{{\left({\frac{{d}}{{d{{x}}}}}{{\left({{\left(\ln{{x}}\right)}{\cdot}{2}}+{1}\right)}}\right)}{x}}}=\\
={{{\left(\ln{{x}}\right)}{\cdot}{2}}+{{1}+{{\left({\frac{{d}}{{d{{x}}}}}{{\left({{\left(\ln{{x}}\right)}{\cdot}{2}}+{1}\right)}}\right)}{x}}}}=\\
={{{\left(\ln{{x}}\right)}{\cdot}{2}}+{{1}+{{\left({{\frac{{d}}{{d{{x}}}}}{{{\left(\ln{{x}}\right)}{\cdot}{2}}}}+{{\frac{{d}}{{d{{x}}}}}{{1}}}\right)}{x}}}}=\\
={{{\left(\ln{{x}}\right)}{\cdot}{2}}+{{1}+{{\left({{2}{\left({\frac{{d}}{{d{{x}}}}}{{\ln{{x}}}}\right)}}+{{\frac{{d}}{{d{{x}}}}}{{1}}}\right)}{x}}}}=\\
={{{\left(\ln{{x}}\right)}{\cdot}{2}}+{{1}+{{\left({{2}{{\left({\frac{{d}}{{d{{x}}}}}{{x}}\right)}{\cdot}{\left(\frac{{1}}{{x}}\right)}}}+{{\frac{{d}}{{d{{x}}}}}{{1}}}\right)}{x}}}}=\\
={{{\left(\ln{{x}}\right)}{\cdot}{2}}+{{1}+{{\left({{2}{\cdot}{{1}{\cdot}{\left(\frac{{1}}{{x}}\right)}}}+{{\frac{{d}}{{d{{x}}}}}{{1}}}\right)}{x}}}}=\\
={{{\left(\ln{{x}}\right)}{\cdot}{2}}+{{1}+{{\left({{2}{\cdot}{\left(\frac{{{1}{\cdot}{1}}}{{x}}\right)}}+{{\frac{{d}}{{d{{x}}}}}{{1}}}\right)}{x}}}}=\\
={{{\left(\ln{{x}}\right)}{\cdot}{2}}+{{1}+{{\left({{2}{\cdot}{\left(\frac{{1}}{{x}}\right)}}+{{\frac{{d}}{{d{{x}}}}}{{1}}}\right)}{x}}}}=\\
={{{\left(\ln{{x}}\right)}{\cdot}{2}}+{{1}+{{\left({\frac{{{2}{\cdot}{1}}}{{x}}}+{{\frac{{d}}{{d{{x}}}}}{{1}}}\right)}{x}}}}=\\
={{{\left(\ln{{x}}\right)}{\cdot}{2}}+{{1}+{{\left({\frac{{2}}{{x}}}+{{\frac{{d}}{{d{{x}}}}}{{1}}}\right)}{x}}}}=\\
={{{\left(\ln{{x}}\right)}{\cdot}{2}}+{{1}+{{\left(\frac{{2}}{{x}}\right)}{x}}}}=\\
={{{\left(\ln{{x}}\right)}{\cdot}{2}}+{{1}+{\frac{{{2}{x}}}{{x}}}}}=\\
={{{\left(\ln{{x}}\right)}{\cdot}{2}}+{{1}+{\frac{{{x}{\cdot}{2}}}{{x}}}}}=\\
={{{\left(\ln{{x}}\right)}{\cdot}{2}}+{{1}+{\frac{{{{1}{\cdot}{2}}{{x}^{\left({1}-{{1}{\cdot}{1}}\right)}}}}{{{1}{{x}^{\left({1}-{{1}{\cdot}{1}}\right)}}}}}}}=\\
={{{\left(\ln{{x}}\right)}{\cdot}{2}}+{{1}+{\frac{{{2}{\cdot}{{1}{{x}^{\left({1}-{{1}{\cdot}{1}}\right)}}}}}{{{1}{{x}^{\left({1}-{{1}{\cdot}{1}}\right)}}}}}}}=\\
={{{\left(\ln{{x}}\right)}{\cdot}{2}}+{{1}+{\frac{{{2}{\cdot}{{1}{{x}^{\left({1}-{1}\right)}}}}}{{{1}{{x}^{\left({1}-{{1}{\cdot}{1}}\right)}}}}}}}=\\
={{{\left(\ln{{x}}\right)}{\cdot}{2}}+{{1}+{\frac{{{2}{\cdot}{{1}{{x}^{\left({-{1}}+{1}\right)}}}}}{{{1}{{x}^{\left({1}-{{1}{\cdot}{1}}\right)}}}}}}}=\\
={{{\left(\ln{{x}}\right)}{\cdot}{2}}+{{1}+{\frac{{{2}{\cdot}{{1}{{x}^{\left(-{0}\right)}}}}}{{{1}{{x}^{\left({1}-{{1}{\cdot}{1}}\right)}}}}}}}=\\
={{{\left(\ln{{x}}\right)}{\cdot}{2}}+{{1}+{\frac{{2}}{{{1}{{x}^{\left({1}-{{1}{\cdot}{1}}\right)}}}}}}}=\\
={{{\left(\ln{{x}}\right)}{\cdot}{2}}+{{1}+{\frac{{2}}{{{1}{{x}^{\left({1}-{1}\right)}}}}}}}=\\
={{{\left(\ln{{x}}\right)}{\cdot}{2}}+{{1}+{\frac{{2}}{{{1}{{x}^{\left({-{1}}+{1}\right)}}}}}}}=\\
={{{\left(\ln{{x}}\right)}{\cdot}{2}}+{{1}+{\frac{{2}}{{{1}{{x}^{\left(-{0}\right)}}}}}}}=\\
={{{\left(\ln{{x}}\right)}{\cdot}{2}}+{{1}+{2}}}=\\
={{{\left(\ln{{x}}\right)}{\cdot}{2}}+{{2}+{1}}}=\\
={{{\left(\ln{{x}}\right)}{\cdot}{2}}+{3}}\end{gather*}
\centering\includegraphics[scale=0.5]{graph.png}
\end{document}